theories/FOL/PA_undec.v
@@ -5,6 +5,27 @@ From Undecidability.H10 Require Import H10p H10p_undec.
 From Undecidability.FOL.Reductions Require Import H10p_to_FA.
 
 
+(* ** Reduction for the axiomatisation PA assuming extensionality of models. *)
+
+Theorem H10_ext_entailment_PA :
+  (exists D (I : interp D), extensional I /\ forall psi rho, PA psi -> rho ⊨ psi) -> H10p_SAT ⪯ ext_entailment_PA.
+Proof.
+  intros (D & I & Hext & H).
+  exists embed. intros E. apply H10p_to_FA_ext_sat.
+Qed.
+
+
+Theorem undecidable_ext_entailment_PA :
+  (exists D (I : interp D), extensional I /\ forall psi rho, PA psi -> rho ⊨ psi) -> undecidable ext_entailment_PA.
+Proof.
+  intros H.
+  refine (undecidability_from_reducibility _ (H10_ext_entailment_PA H)).
+  apply H10p_undec.
+Qed.
+
+
+
+(* ** Reductions for the axiomatisations PAeq and FAeq, which include the axioms for equatlity. *)
 
 Theorem H10_entailment_FA : H10p_SAT ⪯ entailment_FA.
 Proof.
