theories/FOL/Util/FA_facts.v
@@ -200,6 +200,12 @@ Section FA_models.
   Hypothesis FA_model : forall ax rho, List.In ax FA -> rho ⊨ ax.
 
 
+  Notation "x 'i=' y" := (i_atom (P:=Eq) ([x ; y])) (at level 30) : PA_Notation.
+  Notation "'iO'" := (i_func (f:=Zero) (Vector.nil D)) (at level 2) : PA_Notation.
+  Notation "'iσ' d" := (i_func (f:=Succ) (Vector.cons d (Vector.nil D))) (at level 37) : PA_Notation.
+  Notation "x 'i⊕' y" := (i_func (f:=Plus) ([x ; y])) (at level 39) : PA_Notation.
+  Notation "x 'i⊗' y" := (i_func (f:=Mult) ([x ; y])) (at level 38) : PA_Notation.
+
   Fact eval_num sigma n : eval sigma (num n) = iμ n.
   Proof.
     induction n.
@@ -207,6 +213,69 @@ Section FA_models.
     - cbn. now rewrite IHn.
   Qed.  
 
+
+  Lemma add_zero' : forall d : D, iO i⊕ d = d.
+  Proof.
+    intros d.
+    assert (List.In ax_add_zero FA) as H by firstorder.
+    specialize (FA_model ax_add_zero (d.:(fun _ => iO)) H).
+    cbn in FA_model. now apply ext_model.
+  Qed.
+
+  Lemma add_rec' : forall n d : D, iσ n i⊕ d = iσ (n i⊕ d).
+  Proof.
+    intros n d.
+    assert (List.In ax_add_rec FA) as H by firstorder.
+    specialize (FA_model ax_add_rec (d.:(fun _ => iO))  H).
+    cbn in FA_model. now apply ext_model. 
+  Qed.
+
+  Lemma mult_zero' : forall d : D, iO i⊗ d = iO.
+  Proof.
+    intros d.
+    assert (List.In ax_mult_zero FA) as H by firstorder.
+    specialize (FA_model ax_mult_zero (d.:(fun _ => iO)) H).
+    cbn in FA_model. now apply ext_model.
+  Qed.
+
+  Lemma mult_rec' : forall n d : D, iσ d i⊗ n = n i⊕ d i⊗ n.
+  Proof.
+    intros n d.
+    assert (List.In ax_mult_rec FA) as H by firstorder.
+    specialize (FA_model ax_mult_rec (d.:(fun _ => iO)) H).
+    cbn in FA_model. now apply ext_model.
+  Qed.
+
+
+  Corollary add_hom x y : iμ (x + y) = iμ x i⊕ iμ y.
+  Proof.
+    induction x.
+    - now rewrite add_zero'.
+    - change (iσ iμ (x + y) = iσ iμ x i⊕ iμ y).
+      now rewrite add_rec', IHx. 
+  Qed.
+
+  Corollary add_nat_to_model : forall x y z, x + y = z -> (iμ x i⊕ iμ y = iμ z).
+  Proof.
+    intros x y z H. now rewrite <- add_hom, H.
+  Qed.
+
+  Corollary mult_hom x y : iμ (x * y) = iμ x i⊗ iμ y.
+  Proof.
+    induction x.
+    - now rewrite mult_zero'.
+    - change (iμ (y + x * y) = (iσ iμ x) i⊗ iμ y ).
+      now rewrite add_hom, IHx, mult_rec'.
+  Qed.
+
+
+  Corollary mult_nat_to_model : forall z x y, x * y = z -> (iμ x i⊗ iμ y = iμ z).
+  Proof.
+    intros x y z H. now rewrite <- mult_hom, H.
+  Qed.
+
+
+  
 End FA_models.
 
 
